Common/Option.lean
@@ -9,3 +9,10 @@ def unzip : (a : Option (α×β)) → (Option α) × (Option β)
 def toExcept {α : Type u0} {ε : Type u1} { m : Type u0 → Type u2} [Pure m] [MonadExcept m (ε := ε)] (error : ε) : Option α → m α
 | none => throw error
 | some a => pure a
+
+def bindWithProof (o : Option α) (f : (v : α) → (o = some v) → Option β) : Option β :=
+  match o with
+  | .some v => f v rfl
+  | .none => none
+
+def mapWithProof (o : Option α) (f : (v : α) → (o = some v) → β) : Option β := bindWithProof o (some $ f · ·)
